Algolean.lean
@@ -40,5 +40,7 @@ public import Algolean.Models.ReadWriteVec
 public import Algolean.Models.RobertsonWebb
 public import Algolean.Models.SingleTapeTM
 public import Algolean.Models.WordRAM
+public import Algolean.Problems.Basic
+public import Algolean.Problems.Search
 public import Algolean.QueryComposition
 public import Algolean.QueryModel
